Add all of the expression theory files from BSc Honours thesis by Brae Webb

exprs/Base.thy
@@ -1,25 +1,42 @@
-theory Base
-(* These theories of expression trees and rewrite rules
-   come from Brae Webb's BSc honours thesis:
+section "Intermediate Representation"
+text \<open>This defines the IR of expressions and statements
+within a generic imperative programming language.
 
-     "Verifying Semantics Preservation of Optimisation Passes"
-     by Brae Webb
-     School of Information Technology and Electrical Engineering,
-     The University of Queensland,
-     November 2019.
-*)
-imports
-  Main
+Expressions such as multiplication and variable look-up are expressed as nodes
+which evaluate to a primitive value type. An expression node may contain further
+nested expression nodes, forming a tree like structure.
+
+Statements such as if and assignment are expressed as control nodes which store
+their successor control node and any expression nodes they require as input.
+
+The structure of program as a whole is a directed acyclic graph which
+represents both the data flow and control flow of the program.
+
+This is not dis-similar to the Graal IR
+excluding the ability of the Graal IR to have a node pointed to from
+multiple locations as a form of representation optimisation.
+\<close>
+
+theory Base
+  imports
+    Main
 begin
 
+subsection "Values"
+text \<open>
+Primitive data types such as integers and booleans. Undefined values occur during
+an evaluation of non type-correct expressions.
+\<close>
 datatype Value =
   UndefinedValue |
   IntegerValue int |
   BooleanValue bool |
   StringValue string
 
-(* Operations are metadata for nodes, a binary node, for example, needs a BinaryOp *)
-
+subsection "Operations"
+text \<open>
+Operations are metadata for nodes, a binary node, for example, needs a BinaryOp
+\<close>
 datatype UnaryOp =
   AbsOp |
   MinusOp |
@@ -36,33 +53,120 @@ datatype BinaryOp =
   OrOp |
   XorOp
 
-(* Data flow nodes are nodes which represent expressions that can be evaluated. *)
+subsection "Nodes"
+text \<open>
+Data flow nodes are nodes which represent expressions that can be evaluated.
+\<close>
+
+text_raw \<open>\DefineSnippet{ir:data-node}{\<close>
 datatype Node =
   ConstNode Value |
-  BinaryNode BinaryOp (left:Node) (right:Node) |
+  BinaryNode BinaryOp Node Node |
   UnaryNode UnaryOp Node |
-  LookupNode string |
+  LookupNode String.string |
   ConditionalNode Node Node Node
+text_raw \<open>}%EndSnippet\<close>
 
-(* Control flow nodes represent the control structure of a program that
-can be run.  These correspond loosely to statements. *)
+text \<open>
+Control flow nodes are nodes which represent the control structure of a program
+that can be run, these correspond loosely to statements.
+\<close>
+text_raw \<open>\DefineSnippet{ir:control-node}{\<close>
 datatype ControlNode =
   EndNode |
   IfNode Node ControlNode ControlNode |
   WhileNode Node ControlNode ControlNode |
   AssignNode String.string Node ControlNode |
-  WriteNode Node ControlNode 
+  WriteNode Node ControlNode
+text_raw \<open>}%EndSnippet\<close>
 
-
+text_raw \<open>\DefineSnippet{ir:example}{\<close>
 value "(IfNode
   (BinaryNode LessOp (LookupNode ''max'') (LookupNode ''value''))
   (WriteNode (ConstNode (BooleanValue True)) next)
   (WriteNode (ConstNode (BooleanValue False)) next)
-  )"
+)"
+text_raw \<open>}%EndSnippet\<close>
 
 value "(IfNode (ConstNode x) (EndNode) (EndNode))"
 
+subsection "State"
+text \<open>
+State is a type for storing the local variable state of an executing program.
+A state consists of a mapping of identifier strings to values.
+\<close>
+type_synonym State = "String.string \<Rightarrow> Value"
+
+text \<open>The update function inserts a new identifier-value pair into an existing state.\<close>
+fun update :: "String.string \<Rightarrow> Value \<Rightarrow> State \<Rightarrow> State" where
+  "update ident value state = (\<lambda>id2.(if (id2 = ident) then value else state id2))"
+
+text \<open>
+emptyState defines a state with an empty stdout and all other values map to undefined value.
+\<close>
+fun emptyState :: "String.string \<Rightarrow> Value" where
+  "emptyState ident = (
+  if (ident = ''stdout'')
+    then (StringValue '''')
+    else UndefinedValue)"
+
+text \<open>
+A state within this system can be used as in the example below where an empty state
+is used to create an initial state function before a new variable mapping is added.
+
+Later the value of the variable is looked up by calling the resulting state function.
+\<close>
+value "(update answer (IntegerValue 42) emptyState) answer"
 
 
+
+section "Refinement"
+text \<open>
+Definition of a refinement relationship of values.
+
+A refinement relationship here means that either the values are equal or 
+the value being refined is an undefined value.
+
+Every value can be refined by the undefined value. Allowing for rewriting rules
+to account for the possibility of a node evaluating to the UndefinedValue type.
+\<close>
+fun refines :: "Value \<Rightarrow> Value \<Rightarrow> bool" (infixl "\<tturnstile>" 50) where
+  "refines UndefinedValue y = True" |
+  "refines x y = (x = y)"
+
+lemma refines_def:
+  assumes "a \<tturnstile> b"
+  shows "(a = UndefinedValue) \<or> (a = b)"
+  using assms refines.elims(2) by auto
+
+
+section "Evaluation"
+text \<open>Coercion evaluations of values into specific primitive types.\<close>
+locale Eval
+begin
+fun bool :: "Value \<Rightarrow> bool" where
+  "bool (BooleanValue a) = a" |
+  "bool a = False"
+
+fun int :: "Value \<Rightarrow> int" where
+  "int (IntegerValue a) = a" |
+  "int a = -1"
+
+fun int_to_str :: "int \<Rightarrow> string \<Rightarrow> string" where
+  "int_to_str x r = (if (x \<ge> 10) 
+    then (int_to_str (x div 10) ([char_of (48 + x mod 10)] @ r))
+    else ([char_of (48 + x)] @ r))"
+
+fun bool_to_str :: "bool \<Rightarrow> string" where
+  "bool_to_str True = ''True''" |
+  "bool_to_str False = ''False''"
+
+fun str :: "Value \<Rightarrow> string" where
+  "str (IntegerValue a) = (int_to_str a '''')" |
+  "str (BooleanValue a) = (bool_to_str a)" |
+  "str (StringValue a) = a" |
+  "str (UndefinedValue) = ''Undef''"
+
+end
 
 end
