exprs/CodeGen.thy
@@ -1,0 +1,132 @@
+section "Code Generation"
+text \<open>Mechanism for exporting rewriting rules as executable code.\<close>
+
+theory CodeGen
+  imports
+    ExpressionRewrites
+    StatementRewrites
+begin 
+
+typedef TypeCorrectNode = "{node :: Node . (\<forall>s::State . ((eval node s) \<noteq> UndefinedValue))}"
+proof -
+  have "\<exists>n. \<forall>f. eval n f \<noteq> UndefinedValue"
+    by (metis (full_types) Value.simps(6) eval.simps(1))
+  then show ?thesis
+    by blast
+qed
+
+text \<open>
+The Rewrite locale is a series of code lemmas that are translations of the theories
+expressed in the collection of rewriting rules.
+
+As code lemmas need to be in the function form which expresses equality, the
+rewrite locale assumes that no nodes evaluate to UndefinedValue to prove equality.
+This is possible as refinement is defined as the values being equal or one node
+being an UndefinedValue, if we are to assume that no nodes may evaluate to UndefinedValue
+then it is implicitly true given a rewriting rule and this assumption that the
+nodes are semantically equal.
+
+The definition rewrite is used within lemmas to bind the lemma to the rewrite
+definition for code generation.
+\<close>
+text_raw \<open>\DefineSnippet{codegen:rewrite-locale}{\<close>
+locale Rewrite =
+  assumes noUndef: "\<forall> node::Node . \<forall> state::State . (eval node state \<noteq> UndefinedValue)"
+begin
+
+definition rewrite :: "Node \<Rightarrow> Node" where
+  "rewrite Node = Node"
+text_raw \<open>}%EndSnippet\<close>
+
+
+lemma rewrite_conditional_true_code [code]:
+  "rewrite (ConditionalNode (ConstNode (BooleanValue True)) trueBranch falseBranch)
+    = trueBranch"
+  using noUndef rewrite_conditional_true apply auto
+  using refines_def by (meson eval.simps(1))
+
+lemma rewrite_conditional_false_code [code]:
+  "rewrite (ConditionalNode (ConstNode (BooleanValue False)) trueBranch falseBranch)
+    = falseBranch"
+  using noUndef rewrite_conditional_false apply auto
+  using refines_def by (meson eval.simps(1))
+
+lemma rewrite_conditional_equal_code [code]:
+  "rewrite (ConditionalNode (BinaryNode EqualOp a b) c d) = (
+    if (a = c \<and> b = d)
+      then b
+      else (ConditionalNode (BinaryNode EqualOp a b) a b)
+    )"
+  using noUndef rewrite_conditional_equal apply auto
+  using refines_def apply (meson eval.simps(14))
+  using rewrite_def rewrite_conditional_false_code apply force
+  by (meson eval.simps(14))
+  
+lemma rewrite_add_sub_code [code]:
+  "rewrite (BinaryNode AddOp (BinaryNode SubOp x y) z) = (
+    if (y = z)
+      then x
+      else (BinaryNode AddOp (BinaryNode SubOp x y) z)
+    )"
+  using noUndef rewrite_add_sub apply auto
+  using refines_def apply (meson eval.simps(14))
+  by (simp add: rewrite_def)
+
+lemma rewrite_add_sub2_code [code]:
+  "rewrite (BinaryNode AddOp x (BinaryNode SubOp y z)) = (
+    if (x = z)
+      then y
+      else (BinaryNode AddOp x (BinaryNode SubOp y z))
+    )"
+  using noUndef rewrite_add_sub2 apply auto
+  using refines_def apply (meson eval.simps(14))
+  by (simp add: rewrite_def)
+
+text_raw \<open>\DefineSnippet{codegen:lemma-example}{\<close>
+lemma rewrite_neutral_add_code [code]:
+  "rewrite (BinaryNode AddOp e (ConstNode (IntegerValue 0))) = e"
+text_raw \<open>}%EndSnippet\<close>
+  using noUndef rewrite_neutral_add apply auto
+  using refines_def by (meson eval.simps(1))
+
+lemma rewrite_neutral_sub_code [code]:
+  "rewrite (BinaryNode SubOp e (ConstNode (IntegerValue 0))) = e"
+  using noUndef rewrite_neutral_sub apply auto
+  using refines_def by (meson eval.simps(1))
+
+lemma rewrite_neutral_or_code [code]:
+  "rewrite (BinaryNode OrOp e (ConstNode (BooleanValue False))) = e"
+  using noUndef rewrite_neutral_or apply auto
+  using refines_def by (meson eval.simps(1))
+
+lemma rewrite_neutral_and_code [code]:
+  "rewrite (BinaryNode AndOp e (ConstNode (BooleanValue True))) = e"
+  using noUndef rewrite_neutral_and apply auto
+  using refines_def by (meson eval.simps(1))
+
+end
+
+text \<open>The interpretation of a rewrite as code cannot be generated for the
+abstract locale.
+
+In order to prove this interpretation we must find a way to express the conditions
+under which no nodes would evaluation to an undefined value, i.e. we need to express
+type correctness of all nodes.
+\<close>
+lemma type_correct:
+  fixes result :: TypeCorrectNode
+  shows "\<forall>s::State . (eval (Rep_TypeCorrectNode result) s) \<noteq> UndefinedValue"
+  using Rep_TypeCorrectNode by auto
+
+interpretation rewrite_interpretation: Rewrite
+  sorry
+
+text \<open>The export code mechanism of Isabelle used to export all rewriting rules
+under the Rewrite locale.
+\<close>
+text_raw \<open>\DefineSnippet{codegen:export}{\<close>
+export_code Rewrite.rewrite in Scala module_name Compiler
+export_code Rewrite.rewrite in Haskell module_name Compiler
+text_raw \<open>}%EndSnippet\<close>
+
+end
