exprs/Evaluation.thy
@@ -1,0 +1,33 @@
+theory Evaluation
+  imports Semantics
+begin
+
+interpretation evaluation: Eval
+  done
+
+interpretation semantics: Semantic
+  done
+
+value "''hello''"
+value "Eval.int_to_str 573 ''''"
+value "Eval.int_to_str 342542523 ''''"
+value "Eval.int_to_str 5342373 ''''"
+value "Eval.int_to_str 3 ''''"
+
+value "(exec (WriteNode (ConstNode (IntegerValue 5)) EndNode) emptyState) x"
+
+value "(exec
+  (WriteNode (ConstNode (StringValue ''The magic number is ''))
+    (WriteNode (ConstNode (IntegerValue 56)) EndNode))
+  emptyState) ''stdout''"
+
+value "(exec
+(AssignNode ''i'' (ConstNode (IntegerValue 0))
+  (WhileNode (BinaryNode LessOp (LookupNode ''i'') (ConstNode (IntegerValue 4)))
+    (AssignNode ''i'' (BinaryNode AddOp (LookupNode ''i'') (ConstNode (IntegerValue 1)))
+    (WriteNode (LookupNode ''i'')
+    (WriteNode (ConstNode (StringValue '' Fight me Emily ''))
+  EndNode)))
+ EndNode)) emptyState) ''stdout''"
+
+end
