exprs/ExpressionRewrites.thy
@@ -1,0 +1,427 @@
+section "Expression Rewriting"
+text \<open>Expressions that can be rewritten as other semantically equivalent expressions.\<close>
+
+theory ExpressionRewrites
+  imports
+    Semantics
+    Monotonic
+    OperatorProperties
+begin 
+
+text \<open>
+A rewrite (\isasymturnstile) is true if one expression can be rewritten by another expression with
+the original semantics preserved.
+\<close>
+fun expression_rewrites :: "Node \<Rightarrow> Node \<Rightarrow> bool" (infixl "\<turnstile>" 50) where
+  "expression_rewrites a b = (\<forall> s :: State . ((eval a s) \<tturnstile> (eval b s)))"
+
+lemma expression_rewrites_def:
+  fixes a b :: Node
+  shows "a \<turnstile> b \<equiv> (\<forall> s :: State . ((eval a s) \<tturnstile> (eval b s)))"
+  by auto
+
+subsection "Subnode Rewrites"
+text \<open>
+Subnode Rewrites are theories for the binary and unary nodes that proof that
+if a subnode, x, can be rewritten by another node, z, then the node can be
+rewritten with the x subnode replaced with the node z.
+\<close>
+theorem binary_left_subnode_rewrite:
+  fixes x y z :: Node
+  fixes op :: BinaryOp
+  assumes "x \<turnstile> z"
+  shows "BinaryNode op x y \<turnstile> BinaryNode op z y"
+proof (cases "op")
+case AddOp
+  then show ?thesis
+    using MonotonicFunctions.add_monotonic assms monotonic_both_def monotonic_left_def by auto
+next
+case SubOp
+  then show ?thesis
+    using MonotonicFunctions.minus_monotonic assms monotonic_both_def monotonic_left_def by auto
+next
+  case MulOp
+  then show ?thesis
+    using MonotonicFunctions.times_monotonic assms monotonic_both_def monotonic_left_def by auto
+next
+  case DivOp
+  then show ?thesis
+    using MonotonicFunctions.divide_monotonic assms monotonic_both_def monotonic_left_def by auto
+next
+  case EqualOp
+  then show ?thesis
+    using MonotonicFunctions.equal_monotonic assms monotonic_left_def by auto
+next
+  case LessOp
+  then show ?thesis
+    using MonotonicFunctions.less_monotonic assms monotonic_both_def monotonic_left_def by auto
+next
+  case AndOp
+  then show ?thesis
+    using MonotonicFunctions.and_monotonic assms monotonic_both_def monotonic_left_def by auto
+next
+  case OrOp
+then show ?thesis
+  using MonotonicFunctions.or_monotonic assms monotonic_both_def monotonic_left_def by auto
+next
+  case XorOp
+  then show ?thesis
+    using MonotonicFunctions.xor_monotonic assms monotonic_both_def monotonic_left_def by auto
+qed
+
+theorem binary_right_subnode_rewrite:
+  fixes x y z :: Node
+  fixes op :: BinaryOp
+  assumes "x \<turnstile> z"
+  shows "BinaryNode op y x \<turnstile> BinaryNode op y z"
+proof (cases "op")
+case AddOp
+  then show ?thesis
+    using MonotonicFunctions.add_monotonic assms monotonic_both_def monotonic_right_def by auto
+next
+case SubOp
+  then show ?thesis
+    using MonotonicFunctions.minus_monotonic assms monotonic_both_def monotonic_right_def by auto
+next
+  case MulOp
+  then show ?thesis
+    using MonotonicFunctions.times_monotonic assms monotonic_both_def monotonic_right_def by auto
+next
+  case DivOp
+  then show ?thesis
+    using MonotonicFunctions.divide_monotonic assms monotonic_both_def monotonic_right_def by auto
+next
+  case EqualOp
+  then show ?thesis
+    using MonotonicFunctions.equal_monotonic assms monotonic_right_def by auto
+next
+  case LessOp
+  then show ?thesis
+    using MonotonicFunctions.less_monotonic assms monotonic_both_def monotonic_right_def by auto
+next
+  case AndOp
+  then show ?thesis
+    using MonotonicFunctions.and_monotonic assms monotonic_both_def monotonic_right_def by auto
+next
+  case OrOp
+then show ?thesis
+  using MonotonicFunctions.or_monotonic assms monotonic_both_def monotonic_right_def by auto
+next
+  case XorOp
+  then show ?thesis
+    using MonotonicFunctions.xor_monotonic assms monotonic_both_def monotonic_right_def by auto
+qed
+
+theorem unary_refines_subnode:
+  fixes x y :: Node
+  fixes op :: UnaryOp
+  assumes refines: "x \<turnstile> y"
+  shows "UnaryNode op x \<turnstile> UnaryNode op y"
+proof (cases "op")
+case AbsOp
+  then show ?thesis
+    using MonotonicFunctions.abs_monotonic assms monotonic_def by auto
+next
+case MinusOp
+  then show ?thesis
+    using MonotonicFunctions.uminus_monotonic assms monotonic_def by auto
+next
+  case NotOp
+  then show ?thesis
+    using MonotonicFunctions.not_monotonic assms monotonic_def by auto
+qed
+
+
+lemma reflexive_refinement:
+  fixes v :: Value
+  shows "v \<tturnstile> v"
+  using refines.elims(3) by auto
+  
+subsection "Conditional Node Rewrites"
+lemma negation:
+  assumes "(eval x s) = (BooleanValue val)"
+  shows "(Eval.bool (eval (UnaryNode NotOp x) s)) = (\<not>(Eval.bool (eval x s)))"
+  by (simp add: Eval.bool.simps(1) Semantic.logicNot.simps(1) assms)
+
+theorem rewrite_conditional_negated:
+  fixes trueExp falseExp :: Node
+  assumes nc: "\<forall> s :: State . (eval x s = BooleanValue val)"
+  shows
+  "(ConditionalNode (UnaryNode NotOp x) trueExp falseExp)
+    \<turnstile> (ConditionalNode x falseExp trueExp)"
+  using nc negation refines.elims(3) by fastforce
+
+theorem rewrite_conditional_equal_xy:
+  fixes cond x :: Node
+  shows "(ConditionalNode cond x x) \<turnstile> (x)"
+  by (simp add: reflexive_refinement)
+
+theorem rewrite_conditional_true:
+  fixes trueExp falseExp :: Node
+  shows
+  "(ConditionalNode (ConstNode (BooleanValue True)) trueExp falseExp)
+    \<turnstile> trueExp"
+  using refines.elims(3)
+  by (simp add: Eval.bool.simps(1) reflexive_refinement)
+
+theorem rewrite_conditional_false:
+  fixes trueExp falseExp :: Node
+  shows
+  "(ConditionalNode (ConstNode (BooleanValue False)) trueExp falseExp)
+    \<turnstile> falseExp"
+  using rewrite_conditional_true
+  by (simp add: Eval.bool.simps(1))
+
+lemma either_or:
+  fixes a :: Node
+  shows "(ConditionalNode (BinaryNode EqualOp a a) a a) \<turnstile> a"
+  using reflexive_refinement by simp
+
+lemma equal_node_refinement:
+  fixes a b :: Node
+  fixes s :: State
+  assumes nc: "(eval (BinaryNode EqualOp a b) s) = (BooleanValue True)"
+  shows "(eval a s) \<tturnstile> (eval b s)"
+proof - 
+  have "(eval (BinaryNode EqualOp a b) s) \<tturnstile> (Semantic.equal (eval a s) (eval b s))" using nc by auto
+  then have "((eval (BinaryNode EqualOp a b) s) \<tturnstile> (BooleanValue ((eval a s) = (eval b s))))
+            \<or> ((eval (BinaryNode EqualOp a b) s) \<tturnstile> (UndefinedValue))"
+    by (cases "eval a s"; cases "eval b s"; simp add: Semantic.equal.simps)
+  then show ?thesis
+    using nc
+    by (simp add: reflexive_refinement)
+qed
+
+theorem rewrite_conditional_equal:
+  fixes a b :: Node
+  shows "(ConditionalNode (BinaryNode EqualOp a b) a b) \<turnstile> b"
+  using either_or apply auto
+  using equal_node_refinement
+  by (metis (full_types) Eval.bool.elims(2) eval.simps(6))
+
+
+subsection "Binary Node Rewrites"
+lemma demorgans:
+  shows "(Semantic.logicAnd (Semantic.logicNot x) (Semantic.logicNot y))
+  \<tturnstile> (Semantic.logicNot (Semantic.logicOr x y))"
+  apply (cases x; cases y; simp)
+  by (simp add: Semantic.logicAnd.simps Semantic.logicNot.simps Semantic.logicOr.simps)+
+
+theorem rewrite_demorgans:
+  shows "(BinaryNode AndOp (UnaryNode NotOp x) (UnaryNode NotOp y))
+  \<turnstile> (UnaryNode NotOp (BinaryNode OrOp x y))"
+  using demorgans by simp
+
+theorem rewrite_add_sub:
+  fixes x y :: Node
+  shows "(BinaryNode AddOp (BinaryNode SubOp x y) y) \<turnstile> x"
+  apply auto
+proof -
+  fix s :: State
+  show "Semantic.add (Semantic.sub (eval x s) (eval y s)) (eval y s) \<tturnstile> eval x s"
+    by (cases "eval x s"; cases "eval y s"; simp add: Semantic.sub.simps Semantic.add.simps)
+qed
+
+theorem rewrite_add_sub2:
+  fixes x y :: Node
+  shows "BinaryNode AddOp x (BinaryNode SubOp y x) \<turnstile> y"
+  apply auto
+proof -
+  fix s :: State
+  show "Semantic.add (eval x s) (Semantic.sub (eval y s) (eval x s)) \<tturnstile> eval y s"
+    by (cases "eval x s"; cases "eval y s"; simp add: Semantic.add.simps Semantic.sub.simps)
+qed
+
+subsubsection "Binary Right Constant Shift"
+text "Binary right shift rewriting rule is a canonicalisation rule for shifting
+all constant nodes to the right subnode of binary operations."
+theorem binary_right_shift:
+  assumes one_const: "y \<noteq> ConstNode val"
+  assumes commutative: "commutative op"
+  shows "BinaryNode op (ConstNode const) y \<turnstile> BinaryNode op y (ConstNode const)"
+proof (cases op)
+case AddOp
+  then show ?thesis using add_commutative by simp
+next
+  case SubOp
+  then show ?thesis
+    using commutative by simp
+next
+  case MulOp
+  then show ?thesis using mul_commutative by simp
+next
+  case DivOp
+  then show ?thesis
+    using commutative by simp
+next
+  case EqualOp
+  then show ?thesis
+    using commutative by simp
+next
+  case LessOp
+  then show ?thesis
+    using commutative by simp
+next
+  case AndOp
+  then show ?thesis using and_commutative by simp
+next
+  case OrOp
+  then show ?thesis using or_commutative by simp
+next
+  case XorOp
+  then show ?thesis using xor_commutative by simp
+qed
+
+subsection "Unary Node Rewrites"
+text_raw \<open>\DefineSnippet{rewrite:abs}{\<close>
+lemma nested_abs:
+  assumes "e = (IntegerValue val)"
+  shows "Semantic.abs (Semantic.abs e) \<tturnstile> Semantic.abs e"
+  by (cases "val < 0"; simp add: Semantic.abs.simps(1) assms)
+
+theorem rewrite_nested_abs:
+  fixes e :: Node
+  shows "(UnaryNode AbsOp (UnaryNode AbsOp e)) \<turnstile> (UnaryNode AbsOp e)"
+  using nested_abs
+  by (metis Semantic.abs.elims Semantic.abs.simps(2) eval.simps(13) expression_rewrites.simps refines.elims(3))
+text_raw \<open>}%EndSnippet\<close>
+
+
+lemma nested_minus:
+  assumes "e = (IntegerValue val)"
+  shows "Semantic.uminus (Semantic.uminus e) \<tturnstile> e"
+  by (simp add: Semantic.uminus.simps(1) assms)
+
+theorem rewrite_nested_minus:
+  fixes e :: Node
+  shows "(UnaryNode MinusOp (UnaryNode MinusOp e)) \<turnstile> e"
+  using nested_minus
+  by (metis Semantic.uminus.elims Value.distinct(1) Value.distinct(3) Value.distinct(5) eval.simps(11) expression_rewrites.simps refines.elims(3))
+
+lemma nested_not:
+  assumes "e = (BooleanValue val)"
+  shows "Semantic.logicNot (Semantic.logicNot e) = e"
+  by (simp add: Semantic.logicNot.simps(1) assms)
+
+theorem rewrite_nested_not:
+  fixes e :: Node
+  shows "(UnaryNode NotOp (UnaryNode NotOp e)) \<turnstile> e"
+  apply (simp add: nested_not)
+  by (metis Semantic.logicNot.elims Semantic.logicNot.simps(2) nested_not refines.simps(1) reflexive_refinement)
+
+
+subsection "Neutral Constants"
+text \<open>Rewrite rules that deal with neutral constant in expressions.\<close>
+
+theorem rewrite_neutral_add:
+  fixes e :: Node
+  shows "BinaryNode AddOp e (ConstNode (IntegerValue 0)) \<turnstile> e"
+  apply auto
+proof -
+  fix s :: State
+  show "Semantic.add (eval e s) (IntegerValue 0) \<tturnstile> eval e s"
+    by (cases "eval e s"; simp add: Semantic.add.simps)
+qed
+
+theorem rewrite_neutral_sub:
+  fixes e :: Node
+  shows "(BinaryNode SubOp e (ConstNode (IntegerValue 0))) \<turnstile> e"
+  apply auto
+proof -
+  fix s :: State
+  show "Semantic.sub (eval e s) (IntegerValue 0) \<tturnstile> eval e s"
+    by (cases "eval e s"; simp add: Semantic.sub.simps)
+qed
+
+theorem rewrite_neutral_mul:
+  fixes e :: Node
+  shows "(BinaryNode MulOp e (ConstNode (IntegerValue 1))) \<turnstile> e"
+  apply auto
+proof -
+  fix s :: State
+  show "Semantic.mul (eval e s) (IntegerValue 1) \<tturnstile> eval e s"
+    by (cases "eval e s"; simp add: Semantic.mul.simps)
+qed
+
+theorem rewrite_neutral_div:
+  fixes e :: Node
+  shows "(BinaryNode DivOp e (ConstNode (IntegerValue 1))) \<turnstile> e"
+  apply auto
+proof -
+  fix s :: State
+  show "Semantic.divide (eval e s) (IntegerValue 1) \<tturnstile> eval e s"
+    by (cases "eval e s"; simp add: Semantic.divide.simps)
+qed
+
+theorem rewrite_neutral_or:
+  fixes e :: Node
+  shows "(BinaryNode OrOp e (ConstNode (BooleanValue False))) \<turnstile> e"
+  apply auto
+proof -
+  fix s :: State
+  show "Semantic.logicOr (eval e s) (BooleanValue False) \<tturnstile> eval e s"
+    by (cases "eval e s"; simp add: Semantic.logicOr.simps)
+qed
+
+theorem rewrite_neutral_and:
+  fixes e :: Node
+  shows "(BinaryNode AndOp e (ConstNode (BooleanValue True))) \<turnstile> e"
+  apply auto
+proof -
+  fix s :: State
+  show "Semantic.logicAnd (eval e s) (BooleanValue True) \<tturnstile> eval e s"
+    by (cases "eval e s"; simp add: Semantic.logicAnd.simps)
+qed
+
+subsection "Constant Folding"
+text "Constant folding is the elimination of expressions where all values are constant"
+
+theorem rewrite_fold_add:
+  fixes x y :: int
+  shows "(BinaryNode AddOp (ConstNode (IntegerValue x)) (ConstNode (IntegerValue y))) \<turnstile> ConstNode (IntegerValue (x + y))"
+  using eval.simps
+  by (simp add: Semantic.add.simps(1))
+
+theorem rewrite_fold_sub:
+  fixes x y :: int
+  shows "(BinaryNode SubOp (ConstNode (IntegerValue x)) (ConstNode (IntegerValue y))) \<turnstile> ConstNode (IntegerValue (x - y))"
+  using eval.simps
+  by (simp add: Semantic.sub.simps(1))
+
+theorem rewrite_fold_mul:
+  fixes x y :: int
+  shows "(BinaryNode MulOp (ConstNode (IntegerValue x)) (ConstNode (IntegerValue y))) \<turnstile> ConstNode (IntegerValue (x * y))"
+  using eval.simps
+  by (simp add: Semantic.mul.simps(1))
+
+theorem rewrite_fold_div:
+  fixes x y :: int
+  shows "(BinaryNode DivOp (ConstNode (IntegerValue x)) (ConstNode (IntegerValue y))) \<turnstile> ConstNode (IntegerValue (x div y))"
+  using eval.simps
+  by (simp add: Semantic.divide.simps(1))
+
+theorem rewrite_fold_less:
+  fixes x y :: int
+  shows "(BinaryNode LessOp (ConstNode (IntegerValue x)) (ConstNode (IntegerValue y))) \<turnstile> ConstNode (BooleanValue (x < y))"
+  using eval.simps
+  by (simp add: Semantic.less.simps(1))
+
+theorem rewrite_fold_and:
+  fixes x y :: bool
+  shows "(BinaryNode AndOp (ConstNode (BooleanValue x)) (ConstNode (BooleanValue y))) \<turnstile> ConstNode (BooleanValue (x \<and> y))"
+  using eval.simps
+  by (simp add: Semantic.logicAnd.simps(1))
+
+theorem rewrite_fold_or:
+  fixes x y :: bool
+  shows "(BinaryNode OrOp (ConstNode (BooleanValue x)) (ConstNode (BooleanValue y))) \<turnstile> ConstNode (BooleanValue (x \<or> y))"
+  using eval.simps
+  by (simp add: Semantic.logicOr.simps(1))
+
+theorem rewrite_fold_xor:
+  fixes x y :: bool
+  shows "(BinaryNode XorOp (ConstNode (BooleanValue x)) (ConstNode (BooleanValue y))) \<turnstile> ConstNode (BooleanValue ((x \<and> y) \<or> (\<not>x \<and> \<not>y)))"
+  using eval.simps
+  by (simp add: Semantic.logicXor.simps(1))
+
+end
