exprs/Semantics.thy
@@ -1,0 +1,135 @@
+section "Semantics"
+text \<open>Encoding of the semantics for each of the expression and statements nodes.
+
+For expression nodes their semantics are defined by the definition of their associated
+evaluation in the eval function.
+
+For statement nodes their semantics are defined by the definition of their associated
+evaluation in the exec function.
+\<close>
+
+theory Semantics
+  imports
+    Base
+begin 
+
+text \<open>
+Locale collection of functions which represent the semantics of specific expressions.
+\<close>
+locale Semantic
+begin
+fun add :: "Value \<Rightarrow> Value \<Rightarrow> Value" where
+  "add (IntegerValue a) (IntegerValue b) = (IntegerValue (a + b))" |
+  "add a b = (UndefinedValue)"
+
+fun divide :: "Value \<Rightarrow> Value \<Rightarrow> Value" where
+  "divide (IntegerValue a) (IntegerValue b) = (IntegerValue (a div b))" |
+  "divide a b = (UndefinedValue)"
+
+fun mul :: "Value \<Rightarrow> Value \<Rightarrow> Value" where
+  "mul (IntegerValue a) (IntegerValue b) = (IntegerValue (a * b))" |
+  "mul a b = (UndefinedValue)"
+
+fun sub :: "Value \<Rightarrow> Value \<Rightarrow> Value" where
+  "sub (IntegerValue a) (IntegerValue b) = (IntegerValue (a - b))" |
+  "sub a b = (UndefinedValue)"
+
+fun equal :: "Value \<Rightarrow> Value \<Rightarrow> Value" where
+  "equal (IntegerValue a) (IntegerValue b) = (BooleanValue (a = b))" |
+  "equal (BooleanValue a) (BooleanValue b) = (BooleanValue (a = b))" |
+  "equal a b = UndefinedValue"
+
+fun less :: "Value \<Rightarrow> Value \<Rightarrow> Value" where
+  "less (IntegerValue a) (IntegerValue b) = (BooleanValue (a < b))" |
+  "less a b = (UndefinedValue)"
+
+fun logicAnd :: "Value \<Rightarrow> Value \<Rightarrow> Value" where
+  "logicAnd (BooleanValue a) (BooleanValue b) = (BooleanValue (a \<and> b))" |
+  "logicAnd a b = (UndefinedValue)"
+
+fun logicOr :: "Value \<Rightarrow> Value \<Rightarrow> Value" where
+  "logicOr (BooleanValue a) (BooleanValue b) = (BooleanValue (a \<or> b))" |
+  "logicOr a b = (UndefinedValue)"
+
+fun logicXor :: "Value \<Rightarrow> Value \<Rightarrow> Value" where
+  "logicXor (BooleanValue a) (BooleanValue b) 
+      = (BooleanValue ((a \<and> b) \<or> ((\<not>a) \<and> (\<not>b))))" |
+  "logicXor a b = (UndefinedValue)"
+
+
+
+fun uminus :: "Value \<Rightarrow> Value" where
+  "uminus (IntegerValue a) = (IntegerValue (-a))" |
+  "uminus a = (UndefinedValue)"
+
+fun logicNot :: "Value \<Rightarrow> Value" where
+  "logicNot (BooleanValue a) = (BooleanValue (\<not>a))" |
+  "logicNot a = (UndefinedValue)"
+
+fun abs :: "Value \<Rightarrow> Value" where
+  "abs (IntegerValue a) = (
+    if (a < 0)
+      then (IntegerValue (-a))
+      else (IntegerValue a))" |
+  "abs a = (UndefinedValue)"
+
+end
+
+subsection "Expression Evaluation"
+text \<open>
+An evaluation function which evaluates an expression node within a state.
+Uses the semantics defined within the Semantic locale.
+
+The eval function is that function which defines the semantics of expressions.
+\<close>
+fun eval :: "Node \<Rightarrow> State \<Rightarrow> Value" where
+  "eval (ConstNode a) s = a" |
+
+  "eval (BinaryNode AddOp a b) s = (Semantic.add (eval a s) (eval b s))" |
+  "eval (BinaryNode SubOp a b) s = (Semantic.sub (eval a s) (eval b s))" |
+  "eval (BinaryNode MulOp a b) s = (Semantic.mul (eval a s) (eval b s))" |
+  "eval (BinaryNode DivOp a b) s = (Semantic.divide (eval a s) (eval b s))" |
+  "eval (BinaryNode EqualOp a b) s = (Semantic.equal (eval a s) (eval b s))" |
+  "eval (BinaryNode LessOp a b) s = (Semantic.less (eval a s) (eval b s))" |
+  "eval (BinaryNode AndOp a b) s = (Semantic.logicAnd (eval a s) (eval b s))" |
+  "eval (BinaryNode OrOp a b) s = (Semantic.logicOr (eval a s) (eval b s))" |
+  "eval (BinaryNode XorOp a b) s = (Semantic.logicXor (eval a s) (eval b s))" |
+
+  "eval (UnaryNode MinusOp e) s = (Semantic.uminus (eval e s))" |
+  "eval (UnaryNode NotOp e) s = (Semantic.logicNot (eval e s))" |
+  "eval (UnaryNode AbsOp e) s = (Semantic.abs (eval e s))" |
+
+  "eval (LookupNode a) s = (s a)" |
+ 
+  "eval (ConditionalNode cond true false) s =
+    (if (Eval.bool (eval cond s))
+      then (eval true s)
+      else (eval false s))"
+
+
+subsection "Statement Evaluation"
+text \<open>
+Statements or control nodes are evaluated using the exec function which
+executes the node and performs some actions.
+\<close>
+function exec :: "ControlNode \<Rightarrow> State \<Rightarrow> State" where
+  "exec (EndNode) s = s" |
+  "exec (IfNode cond trueBranch falseBranch) s = 
+    (if (Eval.bool (eval cond s)) 
+      then (exec trueBranch s) 
+      else (exec falseBranch s))" |
+  "exec (AssignNode ident expr next) s = (exec next (update ident (eval expr s) s))" |
+  "exec (WriteNode expr next) s = (exec next
+  (update
+    ''stdout''
+    (StringValue ((Eval.str (s ''stdout'')) @ (Eval.str (eval expr s)))) s
+  ))" |
+  "exec (WhileNode cond body next) s = 
+    (if (Eval.bool (eval cond s))
+      then (exec (WhileNode cond body next) (exec body s))
+      else (exec next s))"
+  by (metis ControlNode.exhaust surj_pair) auto
+termination
+  sorry
+
+end
