exprs/Traversal.thy
@@ -1,0 +1,87 @@
+section "Traversal"
+text "Theory for traversals of the IR structure"
+
+theory Traversal
+  imports Semantics
+begin
+
+fun subnodes :: "ControlNode \<Rightarrow> ControlNode set" where
+  "subnodes (EndNode) = {}" |
+  "subnodes (IfNode _ x y) = (subnodes x) \<union> (subnodes y)" |
+  "subnodes (WhileNode _ x y) = (subnodes x) \<union> (subnodes y)" |
+  "subnodes (AssignNode _ _ x) = (subnodes x)" |
+  "subnodes (WriteNode _ x) = (subnodes x)"
+
+fun expression_nodes :: "ControlNode \<Rightarrow> Node set" where
+  "expression_nodes (EndNode) = {}" |
+  "expression_nodes (IfNode x _ _) = {x}" |
+  "expression_nodes (WhileNode x _ _) = {x}" |
+  "expression_nodes (AssignNode _ x _) = {x}" |
+  "expression_nodes (WriteNode x _) = {x}"
+
+fun expressions :: "ControlNode \<Rightarrow> Node list" where
+  "expressions (EndNode) = []" |
+  "expressions (IfNode x true false) = [x] @ (expressions true) @ (expressions false)" |
+  "expressions (WhileNode x body next) = [x] @ (expressions body) @ (expressions next)" |
+  "expressions (AssignNode _ expr next) = [expr] @ (expressions next)" |
+  "expressions (WriteNode x next) = [x] @ (expressions next)"
+
+fun usages :: "Node \<Rightarrow> ControlNode \<Rightarrow> Node list" where
+  "usages node control = [expr . expr <- (expressions control), expr = node]"
+
+fun usage :: "Node \<Rightarrow> ControlNode \<Rightarrow> nat" where
+  "usage node control = size (usages node control)"
+
+fun used :: "Node \<Rightarrow> ControlNode \<Rightarrow> bool" where
+  "used node control = (size (usages node control) > 0)"
+
+fun contains :: "ControlNode \<Rightarrow> ControlNode \<Rightarrow> bool" where
+  "contains search program = (\<exists> node \<in> (subnodes program) . node = search)"
+
+fun ids :: "ControlNode \<Rightarrow> String.string set" where
+  "ids prog = {id :: String.string . (exec prog emptyState)(id) \<noteq> UndefinedValue}"
+
+fun vals :: "ControlNode \<Rightarrow> Value set" where
+  "vals prog = {val :: Value . (\<exists> id \<in> ids(prog) . (exec prog emptyState)(id) = val)}"
+
+lemma "(ids (AssignNode ''r'' (ConstNode (IntegerValue 1)) EndNode)) = {''r'', ''stdout''}"
+  by auto
+
+lemma "(vals (AssignNode ''r'' (ConstNode (IntegerValue 1)) EndNode)) 
+        = {(IntegerValue 1), (StringValue '''')}"
+  by auto
+
+value "(used
+(ConstNode (IntegerValue 1))
+(AssignNode ''r'' (ConstNode (IntegerValue 1)) EndNode)
+)"
+
+value "(used
+(ConstNode (IntegerValue 1))
+(AssignNode ''r'' (ConstNode (IntegerValue 2)) EndNode)
+)"
+
+value "(used
+(ConstNode (IntegerValue 1))
+(AssignNode ''r'' (ConstNode (IntegerValue 2))
+  (WriteNode (ConstNode (IntegerValue 2))
+  (WriteNode (ConstNode (IntegerValue 1))
+  EndNode)))
+)"
+
+value "(usages
+(ConstNode (IntegerValue 1))
+(AssignNode ''r'' (ConstNode (IntegerValue 2))
+  (WriteNode (ConstNode (IntegerValue 1))
+  (WriteNode (ConstNode (IntegerValue 1))
+  EndNode)))
+)"
+
+value "(usage
+(ConstNode (IntegerValue 1))
+(AssignNode ''r'' (ConstNode (IntegerValue 2))
+  (WriteNode (ConstNode (IntegerValue 2))
+  (WriteNode (ConstNode (IntegerValue 1))
+  EndNode)))
+)"
+end
